% Equation 1
\begin{dmath}
{{\frac{W}{P}}}_{t}={{C}}_{t}^{{{\sigma}}}\, {{N}}_{t}^{{{\varphi}}}
\end{dmath}
% Equation 2
\begin{dmath}
{{Q}}_{t}=\frac{{{\beta}}\, \left(\frac{{{C}}_{t+1}}{{{C}}_{t}}\right)^{\left(-{{\sigma}}\right)}\, \frac{{{Z}}_{t+1}}{{{Z}}_{t}}}{{{\Pi}}_{t+1}}
\end{dmath}
% Equation 3
\begin{dmath}
{{R^n}}_{t}=\frac{1}{{{Q}}_{t}}
\end{dmath}
% Equation 4
\begin{dmath}
{{Y}}_{t}={{A}}_{t}\, \left(\frac{{{N}}_{t}}{{{S}}_{t}}\right)^{1-{{\alpha}}}
\end{dmath}
% Equation 5
\begin{dmath}
{{R^n}}_{t}={{\Pi}}_{t+1}\, {{R^{r}}}_{t}
\end{dmath}
% Equation 6
\begin{dmath}
{{C}}_{t}={{Y}}_{t}
\end{dmath}
% Equation 7
\begin{dmath}
\log\left({{A}}_{t}\right)={{\rho_a}}\, \log\left({{A}}_{t-1}\right)+{{\varepsilon_a}}_{t}
\end{dmath}
% Equation 8
\begin{dmath}
\log\left({{Z}}_{t}\right)={{\rho_{z}}}\, \log\left({{Z}}_{t-1}\right)-{{\varepsilon_z}}_{t}
\end{dmath}
% Equation 9
\begin{dmath}
{{\Delta m_q}}_{t}=\log\left(\frac{{{M/P}}_{t}}{{{M/P}}_{t-1}}\, {{\Pi}}_{t}\right)
\end{dmath}
% Equation 10
\begin{dmath}
{{\Delta m_q}}_{t}={{\rho_{\zeta}}}\, {{\Delta m_q}}_{t-1}+{{\varepsilon_m}}_{t}
\end{dmath}
% Equation 11
\begin{dmath}
{{\Delta m^{ann}}}_{t}={{\Delta m_q}}_{t}\, 4
\end{dmath}
% Equation 12
\begin{dmath}
{{mc}}_{t}=\frac{{{\frac{W}{P}}}_{t}}{{{S}}_{t}\, \frac{{{Y}}_{t}\, \left(1-{{\alpha}}\right)}{{{N}}_{t}}}
\end{dmath}
% Equation 13
\begin{dmath}
1={{\theta}}\, {{\Pi}}_{t}^{{{\epsilon}}-1}+\left(1-{{\theta}}\right)\, {{\Pi^*}}_{t}^{1-{{\epsilon}}}
\end{dmath}
% Equation 14
\begin{dmath}
{{S}}_{t}=\left(1-{{\theta}}\right)\, {{\Pi^*}}_{t}^{\frac{\left(-{{\epsilon}}\right)}{1-{{\alpha}}}}+{{\theta}}\, {{\Pi}}_{t}^{\frac{{{\epsilon}}}{1-{{\alpha}}}}\, {{S}}_{t-1}
\end{dmath}
% Equation 15
\begin{dmath}
{{\Pi^*}}_{t}^{1+{{\epsilon}}\, \frac{{{\alpha}}}{1-{{\alpha}}}}=\frac{{{\epsilon}}\, \frac{{{x_1}}_{t}}{{{x_2}}_{t}}\, \left(1-{{\tau}}\right)}{{{\epsilon}}-1}
\end{dmath}
% Equation 16
\begin{dmath}
{{x_1}}_{t}={{mc}}_{t}\, {{Y}}_{t}\, {{Z}}_{t}\, {{C}}_{t}^{\left(-{{\sigma}}\right)}+{{\beta}}\, {{\theta}}\, {{\Pi}}_{t+1}^{{{\epsilon}}+\frac{{{\alpha}}\, {{\epsilon}}}{1-{{\alpha}}}}\, {{x_1}}_{t+1}
\end{dmath}
% Equation 17
\begin{dmath}
{{x_2}}_{t}={{Y}}_{t}\, {{Z}}_{t}\, {{C}}_{t}^{\left(-{{\sigma}}\right)}+{{\beta}}\, {{\theta}}\, {{\Pi}}_{t+1}^{{{\epsilon}}-1}\, {{x_2}}_{t+1}
\end{dmath}
% Equation 18
\begin{dmath}
{{log(Y)}}_{t}=\log\left({{Y}}_{t}\right)
\end{dmath}
% Equation 19
\begin{dmath}
{{log(W/P)}}_{t}=\log\left({{\frac{W}{P}}}_{t}\right)
\end{dmath}
% Equation 20
\begin{dmath}
{{log(N)}}_{t}=\log\left({{N}}_{t}\right)
\end{dmath}
% Equation 21
\begin{dmath}
{{\pi^{ann}}}_{t}=4\, \log\left({{\Pi}}_{t}\right)
\end{dmath}
% Equation 22
\begin{dmath}
{{i^{ann}}}_{t}=4\, \log\left({{R^n}}_{t}\right)
\end{dmath}
% Equation 23
\begin{dmath}
{{r^{r,ann}}}_{t}=4\, \log\left({{R^{r}}}_{t}\right)
\end{dmath}
% Equation 24
\begin{dmath}
{{M/P}}_{t}=\frac{{{Y}}_{t}}{{{R^n}}_{t}^{{{\eta}}}}
\end{dmath}
% Equation 25
\begin{dmath}
{{log(M)}}_{t}=\log\left({{M/P}}_{t}\, {{P}}_{t}\right)
\end{dmath}
% Equation 26
\begin{dmath}
{{\Pi}}_{t}=\frac{{{P}}_{t}}{{{P}}_{t-1}}
\end{dmath}
% Equation 27
\begin{dmath}
{{log(P)}}_{t}=\log\left({{P}}_{t}\right)
\end{dmath}
% Equation 28
\begin{dmath}
{{log(A)}}_{t}=\log\left({{A}}_{t}\right)
\end{dmath}
% Equation 29
\begin{dmath}
{{log(Z)}}_{t}=\log\left({{Z}}_{t}\right)
\end{dmath}
